src/QueryStructure/Automation/Common.v
@@ -19,12 +19,12 @@ Ltac fold_string_hyps :=
 Ltac fold_string_hyps_in H :=
   repeat
     match goal with
-      | H' := String ?R ?R' : _ |- _ =>
-              match type of H with
-                | context [String R R'] => fold H' in H
-              end
+    | H' := String ?R ?R' : _ |- _ =>
+      match type of H with
+      | context [String R R'] => fold H' in H
+      end
 
-      (*| H' := @BoundedIndex ?A ?Bound : _ |- _ =>
+    (*| H' := @BoundedIndex ?A ?Bound : _ |- _ =>
               match type of H with
                 | context [@BoundedIndex A Bound ] => fold H' in H
               end
@@ -43,10 +43,10 @@ Ltac pose_string_hyps :=
   fold_string_hyps;
   repeat
     match goal with
-      | |- context [String ?R ?R'] =>
-        let str := fresh "StringId" in
-        set (String R R') as str in *
-      (*| |- context [@BoundedIndex ?A ?Bound] =>
+    | |- context [String ?R ?R'] =>
+      let str := fresh "StringId" in
+      set (String R R') as str in *
+    (*| |- context [@BoundedIndex ?A ?Bound] =>
         let idx := fresh "BStringId" in
         set (@BoundedIndex A Bound) as idx in *
       | |- context [ ``(?R) ] =>
@@ -66,39 +66,39 @@ Ltac fold_heading_hyps :=
     end.
 
 Ltac fold_heading_hyps_in H :=
-repeat match goal with
-       | [H' := @Build_RawHeading ?n ?heading :  _ |- _] =>
-         match type of H with
-         | context [@Build_RawHeading n heading] => fold H' in H
-         end
-       | [H' := @Build_RawSchema ?heading ?TupleConstr ?RelConstr |- _ ] =>
-         match type of H with
-         | context [@Build_RawSchema heading TupleConstr RelConstr] =>
-           fold H' in H
-         end
-       | [H' := @Build_RawQueryStructureSchema ?n ?qs_schema ?CrossConstr |- _ ] =>
-         match type of H with
-         | context [@Build_QueryStructureSchema ?n ?qs_schema ?CrossConstr] =>
-           fold H' in H
-         end
-       end.
-
-Ltac pose_heading_hyps := idtac.
-(*  fold_heading_hyps;
   repeat match goal with
-           | |- context[@Build_RawHeading ?n ?attrlist] =>
+         | [H' := @Build_RawHeading ?n ?heading :  _ |- _] =>
+           match type of H with
+           | context [@Build_RawHeading n heading] => fold H' in H
+           end
+         | [H' := @Build_RawSchema ?heading ?TupleConstr ?RelConstr |- _ ] =>
+           match type of H with
+           | context [@Build_RawSchema heading TupleConstr RelConstr] =>
+             fold H' in H
+           end
+         | [H' := @Build_RawQueryStructureSchema ?n ?qs_schema ?CrossConstr |- _ ] =>
+           match type of H with
+           | context [@Build_QueryStructureSchema ?n ?qs_schema ?CrossConstr] =>
+             fold H' in H
+           end
+         end.
+
+Ltac pose_heading_hyps :=
+  fold_heading_hyps;
+  repeat match goal with
+         (*| |- context[@Build_RawHeading ?n ?attrlist] =>
              let heading := fresh "heading" in
-             set (@BuildHeading n attrlist) as heading in *
+             set (@Build_RawHeading n attrlist) as heading in * *)
 
-           | |- context [@Build_RawSchema ?heading ?TupleConstr ?RelConstr] =>
-             let sch := fresh "schma" in
-             set (@Build_RawSchema heading TupleConstr RelConstr) as sch in *
+         | |- context [@Build_RawSchema ?heading ?TupleConstr ?RelConstr] =>
+           let sch := fresh "schma" in
+           set (@Build_RawSchema heading TupleConstr RelConstr) as sch in *
 
-           | |- context [@Build_RawQueryStructureSchema ?n ?qs_schema ?CrossConstr] =>
-             let qs_sch := fresh "qs_schma" in
-             set (@Build_RawQueryStructureSchema n qs_schema CrossConstr) as qs_schema in *
+         | |- context [@Build_RawQueryStructureSchema ?n ?qs_schema ?CrossConstr] =>
+           let qs_sch := fresh "qs_schma" in
+           set (@Build_RawQueryStructureSchema n qs_schema CrossConstr) as qs_schema in *
 
-         end. *)
+         end.
 
 
 Ltac subst_all :=
@@ -106,13 +106,13 @@ Ltac subst_all :=
 
 Ltac pose_string_hyps_in H :=
   fold_string_hyps_in H;
-    repeat
-      (let H' := eval unfold H in H in
+  repeat
+    (let H' := eval unfold H in H in
          match H' with
-           | context [String ?R ?R'] =>
-             let str := fresh "StringId" in
-             set (String R R') as str in *
-           (*| context [@BoundedIndex ?A ?Bound] =>
+         | context [String ?R ?R'] =>
+           let str := fresh "StringId" in
+           set (String R R') as str in *
+         (*| context [@BoundedIndex ?A ?Bound] =>
              let idx := fresh "BStringId" in
              set (@BoundedIndex A Bound) as idx in *
            | context [ ``(?R) ] =>
@@ -123,64 +123,103 @@ Ltac pose_string_hyps_in H :=
              set (@Build_BoundedIndex A Bound idx bnd) as idx in * *)
          end).
 
-Ltac pose_heading_hyps_in H := idtac.
-(*fold_heading_hyps_in H;
+Ltac pose_heading_hyps_in H :=
+  fold_heading_hyps_in H;
   repeat
     (let H' := eval unfold H in H in
          match H' with
-           | context[Build_RawHeading ?n ?attrlist] =>
+         (* | context[Build_RawHeading ?n ?attrlist] =>
              let heading := fresh "heading" in
-             set (@BuildHeading n attrlist) as heading in *
+             set (@Build_RawHeading n attrlist) as heading in * *)
 
-           | context [@Build_RawSchema ?heading ?TupleConstr ?RelConstr] =>
-             let sch := fresh "schma" in
-             set (@Build_RawSchema heading TupleConstr RelConstr) as sch in *
+         | context [@Build_RawSchema ?heading ?TupleConstr ?RelConstr] =>
+           let sch := fresh "schma" in
+           set (@Build_RawSchema heading TupleConstr RelConstr) as sch in *
 
-           | context [@Build_RawQueryStructureSchema ?n ?qs_schema ?CrossConstr] =>
-             let qs_sch := fresh "qs_schma" in
-             set (@Build_QueryStructureSchema n qs_schema CrossConstr) as qs_schema in *
-         end). *)
+         | context [@Build_RawQueryStructureSchema ?n ?qs_schema ?CrossConstr] =>
+           let qs_sch := fresh "qs_schma" in
+           set (@Build_QueryStructureSchema n qs_schema CrossConstr) as qs_schema in *
+         end).
 
 Ltac pose_search_term_in H :=
   repeat
     (let H' := eval unfold H in H in
          match H' with
-           | context[BuildIndexSearchTerm ?Indexes] =>
-             let search_term := fresh "SearchTerm" in
-             set (BuildIndexSearchTerm Indexes) as search_term in *
+         | context[BuildIndexSearchTerm ?Indexes] =>
+           let search_term := fresh "SearchTerm" in
+           set (BuildIndexSearchTerm Indexes) as search_term in *
          end).
 
-  Ltac pose_SearchUpdateTerms_in H :=
-    repeat
-      (let H' := eval unfold H in H in
-           match H' with
-             | context [@Build_SearchUpdateTerms
-                          ?heading
-                          ?search_term ?matcher
-                          ?update_term ?applier] =>
-               let search_update_term := fresh "SearchUpdateTerm" in
-               set (@Build_SearchUpdateTerms heading search_term
-                                             matcher update_term applier)
-                 as search_update_term in *
-           end).
+Ltac pose_SearchUpdateTerms_in H :=
+  repeat
+    (let H' := eval unfold H in H in
+         match H' with
+         | context [@Build_SearchUpdateTerms
+                      ?heading
+                      ?search_term ?matcher
+                      ?update_term ?applier] =>
+           let search_update_term := fresh "SearchUpdateTerm" in
+           set (@Build_SearchUpdateTerms heading search_term
+                                         matcher update_term applier)
+             as search_update_term in *
+         end).
 
-  Ltac zeta_expand id H :=
-    revert id H;
-    match goal with
-        |- let id := ?Z in
-           let H := ?bod in
-           _ =>
-        let H' := fresh in
-        pose (let id := Z in bod) as H;
-          intros id H'; change H' with H in *;
-          clear H'; revert id
-    end.
-  Ltac zeta_expand_all impl :=
-    repeat match goal with
-               H := _ : _, impl := _ : _ |- _ =>
-                                   zeta_expand H impl
-           end.
+Ltac pose_search_term :=
+  repeat
+    ( match goal with
+        |- context[BuildIndexSearchTerm ?Indexes] =>
+        let search_term := fresh "SearchTerm" in
+        set (BuildIndexSearchTerm Indexes) as search_term in *
+      end).
 
+Ltac pose_SearchUpdateTerms :=
+  repeat
+    (match goal with
+       |- context [@Build_SearchUpdateTerms
+                     ?heading
+                     ?search_term ?matcher
+                     ?update_term ?applier] =>
+       let search_update_term := fresh "SearchUpdateTerm" in
+       set (@Build_SearchUpdateTerms heading search_term
+                                     matcher update_term applier)
+         as search_update_term in *
+     end).
+
+Ltac pose_headings_all :=
+  fold_heading_hyps;
+  repeat match goal with
+         | |- context[@Build_RawHeading ?n ?attrlist] =>
+           let heading := fresh "heading" in
+           set (@Build_RawHeading n attrlist) as heading in *
+
+         | |- context [@Build_RawSchema ?heading ?TupleConstr ?RelConstr] =>
+           let sch := fresh "schma" in
+           set (@Build_RawSchema heading TupleConstr RelConstr) as sch in *
+
+         | |- context [@Build_RawQueryStructureSchema ?n ?qs_schema ?CrossConstr] =>
+           let qs_sch := fresh "qs_schma" in
+           set (@Build_RawQueryStructureSchema n qs_schema CrossConstr) as qs_schema in *
+         end.
+
+
+
+Ltac zeta_expand id H :=
+  revert id H;
+  match goal with
+    |- let id := ?Z in
+       let H := ?bod in
+       _ =>
+    let H' := fresh in
+    pose (let id := Z in bod) as H;
+      intros id H'; change H' with H in *;
+      clear H'; revert id
+  end.
+
+Ltac zeta_expand_all impl :=
+  repeat match goal with
+           H := _ : _, impl := _ : _ |- _ =>
+           zeta_expand H impl
+         end.
 
 Ltac CombineCase1 x y :=
   fun a => x a y.
@@ -229,9 +268,9 @@ Ltac CombineIndexTactics IndexPackage1 IndexPackage2 f :=
               ltac:(fun matchIndex1 IndexUse1 createEarlyTerm1 createLastTerm1
                         IndexUse_dep1 createEarlyTerm_dep1 createLastTerm_dep1 =>
                       f ltac:(CombineCase2 matchIndex1 matchIndex2)
-                        ltac:(CombineCase5 IndexUse1 IndexUse2)
-                        ltac:(CombineCase10 createEarlyTerm1 createEarlyTerm2)
-                        ltac:(CombineCase7 createLastTerm1 createLastTerm2)
-                        ltac:(CombineCase7 IndexUse_dep1 IndexUse_dep2)
-                        ltac:(CombineCase11 createEarlyTerm_dep1 createEarlyTerm_dep2)
-                        ltac:(CombineCase8 createLastTerm_dep1 createLastTerm_dep2))).
+                               ltac:(CombineCase5 IndexUse1 IndexUse2)
+                                      ltac:(CombineCase10 createEarlyTerm1 createEarlyTerm2)
+                                             ltac:(CombineCase7 createLastTerm1 createLastTerm2)
+                                                    ltac:(CombineCase7 IndexUse_dep1 IndexUse_dep2)
+                                                           ltac:(CombineCase11 createEarlyTerm_dep1 createEarlyTerm_dep2)
+                                                                  ltac:(CombineCase8 createLastTerm_dep1 createLastTerm_dep2))).
